Tests/DTLC/TrmSpec.lean
@@ -7,129 +7,32 @@ namespace Trm
 open Lp2lc.Active.Util
 open Lp2lc.Active.DTLC
 open Lp2lc.Active.DTLC.Symbolic
-open Lp2lc.Active.DTLC.Runtime
+open TypeHinted
 
 section eraseType
 
 example :
-    (annotatedFalse : Trm).type.eraseRecursively =
+    (annotatedFalse : Trm).typeHint.eraseRecursively =
       (false : Trm) := rfl
 
 example :
-    (annotatedIdFn : Trm).type.eraseRecursively =
+    (annotatedIdFn : Trm).typeHint.eraseRecursively =
       .val (.fn fun x => .ref x) := rfl
 
 example :
-    (annotatedIdFnOnFalse : Trm).type.eraseRecursively =
+    (annotatedIdFnOnFalse : Trm).typeHint.eraseRecursively =
       .apply
-        (annotatedIdFn : Trm).type.eraseRecursively
+        (annotatedIdFn : Trm).typeHint.eraseRecursively
         (false : Trm) := rfl
 
 end eraseType
-
--- section compile
-
--- example [Compiletime.Env Symbol] :
---     ((false : Trm).compile 0) = .outOfFuel := rfl
-
--- example [Compiletime.Env Symbol] :
---     ((false : Trm).compile 1) =
---       .result ((false : Trm).type.eraseRecursively) := rfl
-
--- example [Compiletime.Env Symbol] :
---     ((true : Trm).compile 1) =
---       .result ((true : Trm).type.eraseRecursively) := rfl
-
--- example [Compiletime.Env Symbol] :
---     ((idFn : Trm).compile 1) =
---       .result ((idFn : Trm).type.eraseRecursively) := rfl
-
--- example [Compiletime.Env Symbol] :
---     ((idFnOnFalse : Trm).compile 2) =
---       .result
---         (.apply
---           (idFn : Trm).type.eraseRecursively
---           (false : Trm).type.eraseRecursively) := rfl
-
--- example [Compiletime.Env Symbol] :
---     ((get1st : Trm).compile 1) =
---       .result ((get1st : Trm).type.eraseRecursively) := rfl
-
--- example [Compiletime.Env Symbol] :
---     ((get2nd : Trm).compile 1) =
---       .result ((get2nd : Trm).type.eraseRecursively) := rfl
-
--- example [Compiletime.Env Symbol] :
---     ((get1stOnTuple : Trm).compile 3) =
---       .result ((get1stOnTuple : Trm).type.eraseRecursively) := rfl
-
--- example [Compiletime.Env Symbol] :
---     ((get2ndOnTuple : Trm).compile 3) =
---       .result ((get2ndOnTuple : Trm).type.eraseRecursively) := rfl
-
--- example [Compiletime.Env Symbol] :
---     ((apply1stOn2ndFn : Trm).compile 1) =
---       .result ((apply1stOn2ndFn : Trm).type.eraseRecursively) := rfl
-
--- example [Compiletime.Env Symbol] :
---     ((apply1stOn2ndFnOnTuple : Trm).compile 3) =
---       .result ((apply1stOn2ndFnOnTuple : Trm).type.eraseRecursively) := rfl
-
--- example [Compiletime.Env Symbol] :
---     ((applyidFnOnItself : Trm).compile 2) =
---       .result ((applyidFnOnItself : Trm).type.eraseRecursively) := rfl
-
--- example [Compiletime.Env Symbol] :
---     ((idFnOnFalse2 : Trm).compile 3) =
---       .result ((idFnOnFalse2 : Trm).type.eraseRecursively) := rfl
-
--- example [Compiletime.Env Symbol] :
---     ((Malformed.apply1 : Trm).compile 4) =
---       .error := rfl
-
--- example [Compiletime.Env Symbol] :
---     ((Malformed.primitiveApply : Trm).compile 2) = .error := rfl
-
--- example [Compiletime.Env Symbol] :
---     ((primitiveTrueFn : Trm).compile 1) =
---       .result ((primitiveTrueFn : Trm).type.eraseRecursively) := rfl
-
--- example [Compiletime.Env Symbol] :
---     ((primitiveTrueFnOnFalse : Trm).compile 2) =
---       .result ((primitiveTrueFnOnFalse : Trm).type.eraseRecursively) := rfl
-
--- example [Compiletime.Env Symbol] :
---     ((annotatedFalse : Trm).compile 2) =
---       .result ((annotatedFalse : Trm).type.eraseRecursively) := rfl
-
--- example [Compiletime.Env Symbol] :
---     ((annotatedIdFn : Trm).compile 2) =
---       .result ((annotatedIdFn : Trm).type.eraseRecursively) := rfl
-
--- example [Compiletime.Env Symbol] :
---     ((annotatedIdFnOnFalse : Trm).compile 4) =
---       .result ((annotatedIdFnOnFalse : Trm).type.eraseRecursively) := rfl
-
--- example [Compiletime.Env Symbol] :
---     ((.typeHinted
---       (.val (.primitive "false"))
---       (.depFn .primitive (fun _ => .primitive)) : Trm).compile 2) =
---       .error := rfl
-
--- example [Compiletime.Env Symbol] :
---     ((.typeHinted
---       (.val (.fn (fun x => .ref x)))
---       .primitive : Trm).compile 2) =
---       .error := rfl
-
--- end compile
 
 section eval
 
 @[reducible] unsafe def runtimeCanEval (value : Val) : Permission.Eval Val value :=
   unsafeCast ()
 
-unsafe instance : Env Symbol where
+unsafe instance : Runtime.Env Symbol where
   forVals := {
     save := fun value _permission => unsafeCast value
     load := fun ref => unsafeCast ref
@@ -210,6 +113,122 @@ unsafe example : ((Trm.primitiveTrueFnOnFalse : Trm).eval 2) =
   rfl
 
 end eval
+
+section compile
+
+example [Compiletime.Env Symbol] :
+    false.compile 0 = .outOfFuel := by
+  sorry
+
+example [Compiletime.Env Symbol] :
+    false.compile 1 =
+      .result false := by
+  sorry
+
+example [Compiletime.Env Symbol] :
+    true.compile 1 =
+      .result true := by
+  sorry
+
+example [Compiletime.Env Symbol] :
+    idFn.compile 1 =
+      .result idFn := by
+  sorry
+
+example [Compiletime.Env Symbol] :
+    idFnOnFalse.compile 2 =
+      .result idFnOnFalse := by
+  sorry
+
+example [Compiletime.Env Symbol] :
+    get1st.compile 1 =
+      .result get1st := by
+  sorry
+
+example [Compiletime.Env Symbol] :
+    get2nd.compile 1 =
+      .result get2nd := by
+  sorry
+
+example [Compiletime.Env Symbol] :
+    get1stOnTuple.compile 3 =
+      .result get1stOnTuple := by
+  sorry
+
+example [Compiletime.Env Symbol] :
+    get2ndOnTuple.compile 3 =
+      .result get2ndOnTuple := by
+  sorry
+
+example [Compiletime.Env Symbol] :
+    apply1stOn2ndFn.compile 1 =
+      .result apply1stOn2ndFn := by
+  sorry
+
+example [Compiletime.Env Symbol] :
+    apply1stOn2ndFnOnTuple.compile 3 =
+      .result apply1stOn2ndFnOnTuple := by
+  sorry
+
+example [Compiletime.Env Symbol] :
+    applyidFnOnItself.compile 2 =
+      .result applyidFnOnItself := by
+  sorry
+
+example [Compiletime.Env Symbol] :
+    idFnOnFalse2.compile 3 =
+      .result idFnOnFalse2 := by
+  sorry
+
+example [Compiletime.Env Symbol] :
+    Malformed.apply1.compile 4 =
+      .error := by
+  sorry
+
+example [Compiletime.Env Symbol] :
+    Malformed.primitiveApply.compile 2 = .error := by
+  sorry
+
+example [Compiletime.Env Symbol] :
+    primitiveTrueFn.compile 1 =
+      .result primitiveTrueFn := by
+  sorry
+
+example [Compiletime.Env Symbol] :
+    primitiveTrueFnOnFalse.compile 2 =
+      .result primitiveTrueFnOnFalse := by
+  sorry
+
+example [Compiletime.Env Symbol] :
+    annotatedFalse.compile 2 =
+      .result annotatedFalse.typeHint.eraseRecursively := by
+  sorry
+
+example [Compiletime.Env Symbol] :
+    annotatedIdFn.compile 2 =
+      .result annotatedIdFn.typeHint.eraseRecursively := by
+  sorry
+
+example [Compiletime.Env Symbol] :
+    annotatedIdFnOnFalse.compile 4 =
+      .result annotatedIdFnOnFalse.typeHint.eraseRecursively := by
+  sorry
+
+example [Compiletime.Env Symbol] :
+    ((.typeHinted
+      (.val (.primitive "false"))
+      (.depFn .primitive (fun _ => .primitive)) : Trm).compile 2) =
+      .error := by
+  sorry
+
+example [Compiletime.Env Symbol] :
+    ((.typeHinted
+      (.val (.fn (fun x => .ref x)))
+      .primitive : Trm).compile 2) =
+      .error := by
+  sorry
+
+end compile
 
 end Trm
 
